ILLVarInt.v
@@ -5,9 +5,116 @@ Require Import vars.
 Require Import multiset_spec.
 Require Import multiset.
 Require Import NatOrderedType OrderedTypeEx.
+Require Import Omega ROmega.
+Module N_OT <: OrderedType.
 
-Module N_OT:= UOT_to_OT(Nat_as_OT). (* nat as an OrederedType *)
-Module MILL := ILL_Make(N_OT). (* Build ILL with vars as intergers *)
+  Definition t : Type := nat.
+
+  Definition eq : t -> t -> Prop := eq.
+  Definition lt : t -> t -> Prop := lt.
+
+  Definition eq_refl : forall x : t, eq x x := @eq_refl _.
+  Definition eq_sym : forall x y : t, eq x y -> eq y x := @eq_sym _.
+  Definition eq_trans : forall x y z : t, eq x y -> eq y z -> eq x z := @eq_trans _.
+
+  Definition lt_trans : forall x y z : t, lt x y -> lt y z -> lt x z := Lt.lt_trans.
+  Definition lt_not_eq : forall x y : t, lt x y -> ~ eq x y.
+  Proof.
+    intros x y H. unfold lt,eq  in *; omega.
+  Defined.
+
+  Functional Scheme nat_compare_rect := Induction for nat_compare Sort Type.
+  
+  Definition nat_compare_eq : ∀ n m : nat, nat_compare n m = Eq → n = m.
+  Proof.
+    intros n m.
+    functional induction (nat_compare n m) using nat_compare_rect.
+    intros _;reflexivity.
+    intros abs;discriminate.
+    intros abs;discriminate.
+    intros H;rewrite (IHc H);reflexivity.
+  Defined.
+
+
+  Definition nat_compare_Lt_lt : forall n m, nat_compare n m = Lt -> n<m.
+  Proof.
+    intros n m.
+    functional induction (nat_compare n m) using nat_compare_rect.
+    intros abs;discriminate.
+    intros;zify;romega.
+    intros abs;discriminate.
+    intros H;assert (U:=IHc H).
+    clear IHc H.
+    intros;zify;romega.
+  Defined.
+
+  Lemma nat_compare_Gt_gt : forall n m, nat_compare n m = Gt -> n>m.
+  Proof.
+    intros n m.
+    functional induction (nat_compare n m) using nat_compare_rect.
+    intros abs;discriminate.
+    intros abs;discriminate.
+    intros;zify;romega.
+    intros H;assert (U:=IHc H).
+    clear IHc H.
+    intros;zify;romega.
+  Defined.
+
+  Lemma compare : forall x y : t, Compare lt eq x y.
+  Proof.
+    intros x y; destruct (nat_compare x y) as [ | | ]_eqn.
+    apply EQ. apply nat_compare_eq; assumption.
+    apply LT. apply nat_compare_Lt_lt; assumption.
+    apply GT. apply nat_compare_Gt_gt; assumption.
+    Defined.
+
+  Hint Immediate eq_sym.
+  Hint Resolve eq_refl eq_trans lt_not_eq lt_trans.
+
+  Definition eq_dec : forall x y, { eq x y } + { ~ eq x y }.
+  Proof.
+    unfold eq,t.
+    fix 1; intros [ | x] [ | y].
+    left;reflexivity.
+    right;intro abs;discriminate abs.
+    right;intro abs;discriminate abs.
+    case (eq_dec x y);intros Heq.
+    left;rewrite Heq;reflexivity.
+    right;intros abs;elim Heq;injection abs;intros;assumption.
+  Defined.
+
+End N_OT.
+Module MILL.
+
+  Include  ILL_Make(N_OT). (* Build ILL with vars as intergers *)
+
+  Lemma eq_is_eq : forall f g, eq f g <-> f = g.
+  Proof.
+    intros f.
+    induction f;destruct g;simpl;split;try tauto;try discriminate.
+    intros;subst;try reflexivity.
+    intros H;injection H;tauto.
+    intros [H1 H2].
+    destruct (IHf1 g1) as [h _];rewrite h;try assumption;clear h;
+      destruct (IHf2 g2) as [h _];rewrite h;try assumption;reflexivity.
+    intros H;injection H;clear H;intros;subst;split;apply FormulaOrdered.eq_refl.
+    intros [H1 H2].
+    destruct (IHf1 g1) as [h _];rewrite h;try assumption;clear h;
+      destruct (IHf2 g2) as [h _];rewrite h;try assumption;reflexivity.
+    intros H;injection H;clear H;intros;subst;split;apply FormulaOrdered.eq_refl.
+    intros [H1 H2].
+    destruct (IHf1 g1) as [h _];rewrite h;try assumption;clear h;
+      destruct (IHf2 g2) as [h _];rewrite h;try assumption;reflexivity.
+    intros H;injection H;clear H;intros;subst;split;apply FormulaOrdered.eq_refl.
+    intros H1.
+    destruct (IHf g) as [h _];rewrite h;try assumption;clear h;reflexivity.
+    intros H;injection H;clear H;intros;subst;apply FormulaOrdered.eq_refl.
+    intros [H1 H2].
+    destruct (IHf1 g1) as [h _];rewrite h;try assumption;clear h;
+      destruct (IHf2 g2) as [h _];rewrite h;try assumption;reflexivity.
+    intros H;injection H;clear H;intros;subst;split;apply FormulaOrdered.eq_refl.
+  Qed.
+End MILL.
 Import MILL.
 Import FormulaMultiSet.
 
