emma.v
@@ -104,136 +104,130 @@ Print originelle.
 
 Require Import JMeq.
 
-Program Fixpoint essai (e:env) (f:formula) (h: e ⊢ f) {struct h}: bool := 
+Inductive boolP : Prop := trueP | falseP.
+Program Fixpoint essai (e:env) (f:formula) (h: e ⊢ f) {struct h}: boolP := 
 match h with
-  | Id p => true
+  | Id Γ p x => trueP
   | Impl_R Γ p q x => essai _ _ x
-  | Impl_L Γ Δ p q r x x0 => if essai _ _ x then true else essai _ _ x0
-  | Times_R Γ Δ p q x x0 => false
-  | Times_L Γ p q r x => false
-  | One_R => false
-  | One_L Γ p x => essai _ _ x
-  | And_R Γ p q x x0 => false
-  | And_L_1 Γ p q r x => essai _ _ x
-  | And_L_2 Γ p q r x => essai _ _ x
-  | Oplus_L Γ p q r x x0 => if essai _ _ x then true else essai _ _ x0
+  | Impl_L Γ Δ Δ' p q r _ _  x x0 => if essai _ _ x then trueP else essai _ _ x0
+  | Times_R Γ Δ Δ' p q _ x x0 => falseP
+  | Times_L Γ p q r _ x => falseP
+  | One_R Γ _ => falseP
+  | One_L Γ p _ x => essai _ _ x
+  | And_R Γ p q x x0 => falseP
+  | And_L_1 Γ p q r _ x => essai _ _ x
+  | And_L_2 Γ p q r _ x => essai _ _ x
+  | Oplus_L Γ p q r _ x x0 => if essai _ _ x then trueP else essai _ _ x0
   | Oplus_R_1 Γ p q x => essai _ _ x
   | Oplus_R_2 Γ p q x => essai _ _ x
-  | T_ Γ => false
-  | Zero_ Γ p x => false
-  | Bang_D Γ p q x => essai _ _ x
-  | Bang_C Γ p q x => essai _ _ x
-  | Bang_W Γ p q x => false
-  | Multiset Γ Γ' p x x0 => essai _ _ x0
+  | T_ Γ => falseP
+  | Zero_ Γ p _ => falseP
+  | Bang_D Γ p q _ x => essai _ _ x
+  | Bang_C Γ p q _ x => essai _ _ x
+  | Bang_W Γ p q _ x => falseP
 end.
 
-Eval vm_compute in (essai _ _ originelle).
+
+Eval vm_compute in  (essai _ _ originelle).
 
 (* pas d'application de la règle droite de ⊸ *)
 
-Program Fixpoint no_impl_R (e:env) (f:formula) (h: e ⊢ f) {struct h}: bool := 
+Program Fixpoint no_impl_R (e:env) (f:formula) (h: e ⊢ f) {struct h}: boolP := 
 match h with
-  | Id p => true
-  | Impl_R Γ p q x => false
-  | Impl_L Γ Δ p q r x x0 => if no_impl_R _ _ x then no_impl_R _ _ x0 else false 
-  | Times_R Γ Δ p q x x0 => if no_impl_R _ _ x then no_impl_R _ _ x0 else false 
-  | Times_L Γ p q r x => no_impl_R _ _  x
-  | One_R => true 
-  | One_L Γ p x => no_impl_R _ _ x
-  | And_R Γ p q x x0 => if no_impl_R _ _ x then no_impl_R _ _ x0 else false 
-  | And_L_1 Γ p q r x => no_impl_R _ _ x
-  | And_L_2 Γ p q r x => no_impl_R _ _ x
-  | Oplus_L Γ p q r x x0 => if no_impl_R _ _ x then true else no_impl_R _ _ x0
+  | Id Γ p x => trueP
+  | Impl_R Γ p q x => falseP
+  | Impl_L Γ Δ Δ' p q r _ _  x x0 => if no_impl_R _ _ x then no_impl_R _ _ x0 else falseP 
+  | Times_R Γ Δ Δ' p q _ x x0 => if no_impl_R _ _ x then no_impl_R _ _ x0 else falseP 
+  | Times_L Γ p q r _ x => no_impl_R _ _  x
+  | One_R _ _ => trueP 
+  | One_L Γ p _ x => no_impl_R _ _ x
+  | And_R Γ p q x x0 => if no_impl_R _ _ x then no_impl_R _ _ x0 else falseP 
+  | And_L_1 Γ p q r _ x => no_impl_R _ _ x
+  | And_L_2 Γ p q r _ x => no_impl_R _ _ x
+  | Oplus_L Γ p q r _ x x0 => if no_impl_R _ _ x then trueP else no_impl_R _ _ x0
   | Oplus_R_1 Γ p q x => no_impl_R _ _ x
   | Oplus_R_2 Γ p q x => no_impl_R _ _ x
-  | T_ Γ => true 
-  | Zero_ Γ p x => true 
-  | Bang_D Γ p q x => no_impl_R _ _ x
-  | Bang_C Γ p q x => no_impl_R _ _ x
-  | Bang_W Γ p q x => no_impl_R _ _ x
-  | Multiset Γ Γ' p x x0 =>  no_impl_R _ _ x0
+  | T_ Γ => trueP 
+  | Zero_ Γ p x => trueP 
+  | Bang_D Γ p q _ x => no_impl_R _ _ x
+  | Bang_C Γ p q _ x => no_impl_R _ _ x
+  | Bang_W Γ p q _ x => no_impl_R _ _ x
 end.
 
 Eval vm_compute in (no_impl_R _ _ originelle).
 
 (*  *)
-Require Import Bool.
-Program Fixpoint exists_oplus_on_formula (cont: forall (e1:env) (f1:formula) (h1: e1 ⊢ f1) (e2:env) (f2:formula) (h2: e2 ⊢ f2),bool) (φl φr:formula)  (e:env) (f:formula) (h: e ⊢ f) {struct h}: bool := 
+
+Program Fixpoint exists_oplus_on_formula (cont: forall (e1:env) (f1:formula) (h1: e1 ⊢ f1) (e2:env) (f2:formula) (h2: e2 ⊢ f2),boolP) (φl φr:formula)  (e:env) (f:formula) (h: e ⊢ f) {struct h}: boolP := 
 match h with
-  | Id p => false
+  | Id _ _ p => falseP
   | Impl_R Γ p q x => exists_oplus_on_formula cont φl φr _ _ x
-  | Impl_L Γ Δ p q r x x0 => if exists_oplus_on_formula cont φl φr _ _ x then true else exists_oplus_on_formula cont φl φr _ _ x0
-  | Times_R Γ Δ p q x x0 => if exists_oplus_on_formula cont φl φr _ _ x then true else exists_oplus_on_formula cont φl φr _ _ x0
-  | Times_L Γ p q r x => exists_oplus_on_formula cont φl φr _ _ x
-  | One_R => false
-  | One_L Γ p x => exists_oplus_on_formula cont φl φr _ _ x
-  | And_R Γ p q x x0 => if exists_oplus_on_formula cont φl φr _ _ x then true else exists_oplus_on_formula cont φl φr _ _ x0
-  | And_L_1 Γ p q r x => exists_oplus_on_formula cont φl φr _ _ x
-  | And_L_2 Γ p q r x => exists_oplus_on_formula cont φl φr _ _ x
-  | Oplus_L Γ p q r x x0 => 
+  | Impl_L Γ Δ Δ' p q r _ _ x x0 => if exists_oplus_on_formula cont φl φr _ _ x then trueP else exists_oplus_on_formula cont φl φr _ _ x0
+  | Times_R Γ Δ p q _ _ x x0 => if exists_oplus_on_formula cont φl φr _ _ x then trueP else exists_oplus_on_formula cont φl φr _ _ x0
+  | Times_L Γ p q r _ x => exists_oplus_on_formula cont φl φr _ _ x
+  | One_R _ _  => falseP
+  | One_L Γ p _ x => exists_oplus_on_formula cont φl φr _ _ x
+  | And_R Γ p q x x0 => if exists_oplus_on_formula cont φl φr _ _ x then trueP else exists_oplus_on_formula cont φl φr _ _ x0
+  | And_L_1 Γ p q r _ x => exists_oplus_on_formula cont φl φr _ _ x
+  | And_L_2 Γ p q r _ x => exists_oplus_on_formula cont φl φr _ _ x
+  | Oplus_L Γ p q r _ x x0 => 
     if FormulaOrdered.eq_dec p φl 
       then if FormulaOrdered.eq_dec q φr 
         then cont _ _  x _ _ x0
-        else if exists_oplus_on_formula cont φl φr _ _ x then true else exists_oplus_on_formula cont φl φr _ _ x0
-      else if exists_oplus_on_formula cont φl φr _ _ x then true else exists_oplus_on_formula cont φl φr _ _ x0
+        else if exists_oplus_on_formula cont φl φr _ _ x then trueP else exists_oplus_on_formula cont φl φr _ _ x0
+      else if exists_oplus_on_formula cont φl φr _ _ x then trueP else exists_oplus_on_formula cont φl φr _ _ x0
   | Oplus_R_1 Γ p q x => exists_oplus_on_formula cont φl φr _ _ x
   | Oplus_R_2 Γ p q x => exists_oplus_on_formula cont φl φr _ _ x
-  | T_ Γ => false
-  | Zero_ Γ p x => false
-  | Bang_D Γ p q x => exists_oplus_on_formula cont φl φr _ _ x
-  | Bang_C Γ p q x => exists_oplus_on_formula cont φl φr _ _ x
-  | Bang_W Γ p q x => exists_oplus_on_formula cont φl φr _ _ x
-  | Multiset Γ Γ' p x x0 =>  exists_oplus_on_formula cont φl φr _ _ x0
+  | T_ Γ => falseP
+  | Zero_ Γ p x => falseP
+  | Bang_D Γ p q _ x => exists_oplus_on_formula cont φl φr _ _ x
+  | Bang_C Γ p q _ x => exists_oplus_on_formula cont φl φr _ _ x
+  | Bang_W Γ p q _ x => exists_oplus_on_formula cont φl φr _ _ x
 end.
 
 Program Fixpoint forall_impl_l_on_formula 
-  (cont:forall (e1:env) (f1:formula) (h1: e1 ⊢ f1) (e2:env) (f2:formula) (h2: e2 ⊢ f2), bool) 
-  (φl φr:formula)  (e:env) (f:formula) (h: e ⊢ f) {struct h}: bool := 
+  (cont:forall (e1:env) (f1:formula) (h1: e1 ⊢ f1) (e2:env) (f2:formula) (h2: e2 ⊢ f2), boolP) 
+  (φl φr:formula)  (e:env) (f:formula) (h: e ⊢ f) {struct h}: boolP := 
 match h with
-  | Id p => true
+  | Id _ _ p => trueP
   | Impl_R Γ p q x => forall_impl_l_on_formula cont φl φr _ _ x
-  | Impl_L Γ Δ p q r x x0 => 
+  | Impl_L Γ Δ Δ' p q r _ _ x x0 => 
     if FormulaOrdered.eq_dec p φl 
       then if FormulaOrdered.eq_dec q φr 
-        then cont _ _ x _ _ x0 (*if (cont _ _  x) then false else negb (cont _ _  x0) *)
+        then cont _ _ x _ _ x0 (*if (cont _ _  x) then falseP else negb (cont _ _  x0) *)
         else 
           if forall_impl_l_on_formula cont φl φr _ _ x 
             then forall_impl_l_on_formula cont φl φr _ _ x0
-            else false 
-      else if forall_impl_l_on_formula cont φl φr _ _ x then forall_impl_l_on_formula cont φl φr _ _ x0 else false
-  | Times_R Γ Δ p q x x0 => if forall_impl_l_on_formula cont φl φr _ _ x then forall_impl_l_on_formula cont φl φr _ _ x0 else false 
-  | Times_L Γ p q r x => forall_impl_l_on_formula cont φl φr _ _ x
-  | One_R => true 
-  | One_L Γ p x => forall_impl_l_on_formula cont φl φr _ _ x
-  | And_R Γ p q x x0 => if forall_impl_l_on_formula cont φl φr _ _ x then forall_impl_l_on_formula cont φl φr _ _ x0 else false 
-  | And_L_1 Γ p q r x => forall_impl_l_on_formula cont φl φr _ _ x
-  | And_L_2 Γ p q r x => forall_impl_l_on_formula cont φl φr _ _ x
-  | Oplus_L Γ p q r x x0 => if forall_impl_l_on_formula cont φl φr _ _ x then forall_impl_l_on_formula cont φl φr _ _ x0 else false 
+            else falseP 
+      else if forall_impl_l_on_formula cont φl φr _ _ x then forall_impl_l_on_formula cont φl φr _ _ x0 else falseP
+  | Times_R Γ Δ p q _ _ x x0 => if forall_impl_l_on_formula cont φl φr _ _ x then forall_impl_l_on_formula cont φl φr _ _ x0 else falseP 
+  | Times_L Γ p q r _ x => forall_impl_l_on_formula cont φl φr _ _ x
+  | One_R _ _ => trueP 
+  | One_L Γ p _ x => forall_impl_l_on_formula cont φl φr _ _ x
+  | And_R Γ p q x x0 => if forall_impl_l_on_formula cont φl φr _ _ x then forall_impl_l_on_formula cont φl φr _ _ x0 else falseP 
+  | And_L_1 Γ p q r _ x => forall_impl_l_on_formula cont φl φr _ _ x
+  | And_L_2 Γ p q r _ x => forall_impl_l_on_formula cont φl φr _ _ x
+  | Oplus_L Γ p q r _ x x0 => if forall_impl_l_on_formula cont φl φr _ _ x then forall_impl_l_on_formula cont φl φr _ _ x0 else falseP 
   | Oplus_R_1 Γ p q x => forall_impl_l_on_formula cont φl φr _ _ x
   | Oplus_R_2 Γ p q x => forall_impl_l_on_formula cont φl φr _ _ x
-  | T_ Γ => true
-  | Zero_ Γ p x => true 
-  | Bang_D Γ p q x => forall_impl_l_on_formula cont φl φr _ _ x
-  | Bang_C Γ p q x => forall_impl_l_on_formula cont φl φr _ _ x
-  | Bang_W Γ p q x => forall_impl_l_on_formula cont φl φr _ _ x
-  | Multiset Γ Γ' p x x0 =>  forall_impl_l_on_formula cont φl φr _ _ x0
+  | T_ Γ => trueP
+  | Zero_ Γ p x => trueP 
+  | Bang_D Γ p q _ x => forall_impl_l_on_formula cont φl φr _ _ x
+  | Bang_C Γ p q _ x => forall_impl_l_on_formula cont φl φr _ _ x
+  | Bang_W Γ p q _ x => forall_impl_l_on_formula cont φl φr _ _ x
 end.
+Definition orP (b1 b2:boolP) := if b1 then trueP else b2.
+Definition negP (b:boolP) := if b then falseP else trueP.
 
 Definition not_exists_oplus_on_formula lhs rhs (e1:env) (f1:formula) (h1: e1 ⊢ f1) (e2:env) (f2:formula) (h2: e2 ⊢ f2) := 
-  negb (orb (exists_oplus_on_formula (fun _ _ _ _ _ _ => true) lhs rhs _ _ h1) (exists_oplus_on_formula (fun _ _ _ _ _ _ => true) lhs rhs _ _ h2)).
+  negP (orP (exists_oplus_on_formula (fun _ _ _ _ _ _ => trueP) lhs rhs _ _ h1) (exists_oplus_on_formula (fun _ _ _ _ _ _ => trueP) lhs rhs _ _ h2)).
 
 Eval vm_compute in (forall_impl_l_on_formula (not_exists_oplus_on_formula (G⊸1) (G⊸V)) R E _ _ originelle).
 Eval vm_compute in (forall_impl_l_on_formula (not_exists_oplus_on_formula 1 ((B ⊸ V) & (B ⊸ 1))) G 1 _ _ originelle).
 
-
-
-
-
-
-
 Program Fixpoint exists_AtheseA_on_formula 
-  (cont: forall (e1:env) (f1:formula) (h1: e1 ⊢ f1),bool)
-  (φl φr:formula)  (e:env) (f:formula) (h: e ⊢ f) {struct h}: bool := 
+  (cont: forall (e1:env) (f1:formula) (h1: e1 ⊢ f1),boolP)
+  (φl φr:formula)  (e:env) (f:formula) (h: e ⊢ f) {struct h}: boolP := 
 match h with
   | Oplus_R_1 Γ p q x =>
     if FormulaOrdered.eq_dec p φl
@@ -247,50 +241,318 @@ match h with
         then cont _ _  x
         else exists_AtheseA_on_formula cont φl φr _ _ x
       else exists_AtheseA_on_formula cont φl φr _ _ x
-  | Id p => false
+  | Id _ _ p => falseP
   | Impl_R Γ p q x => exists_AtheseA_on_formula cont φl φr _ _ x
-  | Impl_L Γ Δ p q r x x0 => if exists_AtheseA_on_formula cont φl φr _ _ x then true else exists_AtheseA_on_formula cont φl φr _ _ x0
-  | Times_R Γ Δ p q x x0 => if exists_AtheseA_on_formula cont φl φr _ _ x then true else exists_AtheseA_on_formula cont φl φr _ _ x0
-  | Times_L Γ p q r x => exists_AtheseA_on_formula cont φl φr _ _ x
-  | One_R => false
-  | One_L Γ p x => exists_AtheseA_on_formula cont φl φr _ _ x
-  | And_R Γ p q x x0 => if exists_AtheseA_on_formula cont φl φr _ _ x then true else exists_AtheseA_on_formula cont φl φr _ _ x0
-  | And_L_1 Γ p q r x => exists_AtheseA_on_formula cont φl φr _ _ x
-  | And_L_2 Γ p q r x => exists_AtheseA_on_formula cont φl φr _ _ x
-  | Oplus_L Γ p q r x x0 => if exists_AtheseA_on_formula cont φl φr _ _ x then true else exists_AtheseA_on_formula cont φl φr _ _ x0
-  | T_ Γ => false
-  | Zero_ Γ p x => false
-  | Bang_D Γ p q x => exists_AtheseA_on_formula cont φl φr _ _ x
-  | Bang_C Γ p q x => exists_AtheseA_on_formula cont φl φr _ _ x
-  | Bang_W Γ p q x => exists_AtheseA_on_formula cont φl φr _ _ x
-  | Multiset Γ Γ' p x x0 =>  exists_AtheseA_on_formula cont φl φr _ _ x0
+  | Impl_L Γ Δ Δ' p q r _ _ x x0 => if exists_AtheseA_on_formula cont φl φr _ _ x then trueP else exists_AtheseA_on_formula cont φl φr _ _ x0
+  | Times_R Γ Δ p q _ _ x x0 => if exists_AtheseA_on_formula cont φl φr _ _ x then trueP else exists_AtheseA_on_formula cont φl φr _ _ x0
+  | Times_L Γ p q r _ x => exists_AtheseA_on_formula cont φl φr _ _ x
+  | One_R _ _ => falseP
+  | One_L Γ p _ x => exists_AtheseA_on_formula cont φl φr _ _ x
+  | And_R Γ p q x x0 => if exists_AtheseA_on_formula cont φl φr _ _ x then trueP else exists_AtheseA_on_formula cont φl φr _ _ x0
+  | And_L_1 Γ p q r _ x => exists_AtheseA_on_formula cont φl φr _ _ x
+  | And_L_2 Γ p q r _ x => exists_AtheseA_on_formula cont φl φr _ _ x
+  | Oplus_L Γ p q r _ x x0 => if exists_AtheseA_on_formula cont φl φr _ _ x then trueP else exists_AtheseA_on_formula cont φl φr _ _ x0
+  | T_ Γ => falseP
+  | Zero_ Γ p x => falseP
+  | Bang_D Γ p q _ x => exists_AtheseA_on_formula cont φl φr _ _ x
+  | Bang_C Γ p q _ x => exists_AtheseA_on_formula cont φl φr _ _ x
+  | Bang_W Γ p q _ x => exists_AtheseA_on_formula cont φl φr _ _ x
 end.
 
 
-Eval vm_compute in exists_AtheseA_on_formula (fun _ _ _ => true) A M _ _ originelle.
-Eval vm_compute in exists_AtheseA_on_formula (fun _ _ _ => true) A M _ _ titi.
+Eval vm_compute in exists_AtheseA_on_formula (fun _ _ _ => trueP) A M _ _ originelle.
+Eval vm_compute in exists_AtheseA_on_formula (fun _ _ _ => trueP) A M _ _ titi.
+
+Lemma simple: {P&1, B&1, (V⊸A)&1, (E⊸A)&1,(P⊸M)&1,B ⊸ 1,V}⊢A⊕M.
+Proof with try solve [ apply Id;reflexivity | prove_multiset_eq].
+  and_l_1 B 1.
+  weak_impl_l B 1...
+  one_l.
+  and_l_2 P 1.
+  and_l_2 (E ⊸ A) 1.
+  and_l_2 (P ⊸ M) 1.
+  repeat one_l.
+  and_l_1 (V ⊸ A) 1... (* !D au lieu de WL *)
+  weak_impl_l V A...
+  apply Oplus_R_1...
+Qed.
+Require Import Setoid.
+
+ Notation " x ∈ F " := (mem x F = true) (at level 60): ILL_scope. 
+
+ Lemma env_decomp : ∀ Γ, (Γ == ∅)\/exists φ, exists Γ', Γ==φ::Γ'.
+ Proof.
+   intros Γ.
+   destruct Γ.
+   revert sorted.
+   induction this.
+   left;apply eq_bool_correct;vm_compute;reflexivity.
+
+   right.
+   destruct a.
+   exists f.
+   dependent inversion sorted;clear sorted;subst.
+   destruct (IHthis s);clear IHthis.
+   destruct n.
+   exists ∅.
+   intros y.
+   unfold Maps'.find;simpl.
+   case (FormulaOrdered.compare y f);try reflexivity.
+   intros l.
+   unfold eq,Maps'.Equal in H.
+   unfold Maps'.find in H.
+   rewrite H.
+   vm_compute;reflexivity.
+   exists (add_multiple f n ∅).
+   unfold add;simpl.
+   unfold add_multiple;simpl.  
+   rewrite MapsPtes.F.add_eq_o by apply FormulaOrdered.eq_refl.
+   intros y.
+ 
+   case (FormulaOrdered.eq_dec f y);intros Heq1.
+   rewrite MapsPtes.F.add_eq_o by exact Heq1.
+   unfold Maps'.find.
+   simpl.
+   symmetry in Heq1.
+   case (FormulaOrdered.compare y f).
+   intros.
+   elim (@FormulaOrdered.lt_not_eq _ _ l Heq1).
+   reflexivity.
+   symmetry in Heq1.
+   intros. 
+   elim (@FormulaOrdered.lt_not_eq _ _ l Heq1).
+   rewrite MapsPtes.F.add_neq_o by assumption.
+   rewrite MapsPtes.F.add_neq_o by assumption.
+   rewrite MapsPtes.F.empty_o.
+   unfold Maps'.find.
+   simpl.
+   case (FormulaOrdered.compare y f).
+   intros.
+   reflexivity.
+   intros abs;elim Heq1;rewrite abs;apply FormulaOrdered.eq_refl.
+   apply MapsPtes.F.Empty_m in H.
+   destruct H.
+   clear H.
+   assert (v:= H0 (@Maps'.empty_1 nat));clear H0.
+   destruct this.
+   intros;vm_compute;reflexivity.
+   apply False_ind;clear -v.
+   apply Maps'.is_empty_1 in v.
+   vm_compute;discriminate.
+
+   destruct H as [φ' [Γ'' H]].
+ Admitted.
+
+ Lemma add_singleton_abs : 
+   ∀ (φ φ' φ'':formula) Γ, φ'::φ''::Γ == {φ} -> False.
+ Proof.
+   intros φ φ' φ'' Γ H.
+   case (FormulaOrdered.eq_dec φ φ');intros Heq1.
+   rewrite <- Heq1 in H;clear Heq1.
+   case (FormulaOrdered.eq_dec φ φ'');intros Heq2.
+   rewrite <- Heq2 in H;clear Heq2.
+   clear -H .
+   assert (u:=H φ);clear H.
+   unfold add,add_multiple in u.
+   rewrite MapsPtes.F.empty_o in u.
+   rewrite MapsPtes.F.add_eq_o in u by apply FormulaOrdered.eq_refl.
+   destruct (Maps'.find (elt:=nat) φ Γ) .
+   rewrite MapsPtes.F.add_eq_o in u by apply FormulaOrdered.eq_refl.
+   rewrite MapsPtes.F.add_eq_o in u by apply FormulaOrdered.eq_refl.
+   discriminate.
+   rewrite MapsPtes.F.add_eq_o in u by apply FormulaOrdered.eq_refl.
+   rewrite MapsPtes.F.add_eq_o in u by apply FormulaOrdered.eq_refl.
+   discriminate.
+   assert (u:=H φ'');clear -u Heq2.
+   unfold add,add_multiple in u.
+   rewrite MapsPtes.F.empty_o in u.
+   rewrite MapsPtes.F.add_neq_o in u by (intros abs;elim Heq2;rewrite abs;apply FormulaOrdered.eq_refl).
+   rewrite MapsPtes.F.empty_o in u.
+   destruct (Maps'.find (elt:=nat) φ'' Γ) .
+   rewrite MapsPtes.F.add_neq_o in u by (intros abs;elim Heq2;rewrite abs;apply FormulaOrdered.eq_refl).
+   destruct (Maps'.find (elt:=nat) φ Γ) .
+   rewrite MapsPtes.F.add_neq_o in u by (intros abs;elim Heq2;rewrite abs;apply FormulaOrdered.eq_refl).
+   rewrite MapsPtes.F.add_eq_o in u by apply FormulaOrdered.eq_refl.
+   discriminate.
+   rewrite MapsPtes.F.add_neq_o in u by (intros abs;elim Heq2;rewrite abs;apply FormulaOrdered.eq_refl).
+   rewrite MapsPtes.F.add_eq_o in u by apply FormulaOrdered.eq_refl.
+   discriminate.
+   rewrite MapsPtes.F.add_neq_o in u by (intros abs;elim Heq2;rewrite abs;apply FormulaOrdered.eq_refl).
+   destruct (Maps'.find (elt:=nat) φ Γ) .
+   rewrite MapsPtes.F.add_neq_o in u by (intros abs;elim Heq2;rewrite abs;apply FormulaOrdered.eq_refl).
+   rewrite MapsPtes.F.add_eq_o in u by apply FormulaOrdered.eq_refl.
+   discriminate.
+   rewrite MapsPtes.F.add_neq_o in u by (intros abs;elim Heq2;rewrite abs;apply FormulaOrdered.eq_refl).
+   rewrite MapsPtes.F.add_eq_o in u by apply FormulaOrdered.eq_refl.
+   discriminate.
+   assert (u:=H φ');clear -u Heq1.
+   unfold add,add_multiple in u.
+   rewrite MapsPtes.F.empty_o in u.
+   rewrite MapsPtes.F.add_neq_o in u by (intros abs;elim Heq1;rewrite abs;apply FormulaOrdered.eq_refl).
+   rewrite MapsPtes.F.empty_o in u.
+   destruct (Maps'.find (elt:=nat) φ'' Γ) .
+   case (FormulaOrdered.eq_dec φ' φ'');intros Heq2.
+   rewrite MapsPtes.F.add_eq_o in u by (symmetry;assumption).
+   rewrite MapsPtes.F.add_eq_o in u by apply FormulaOrdered.eq_refl.
+   discriminate.   
+   rewrite MapsPtes.F.add_neq_o in u by (intros abs;elim Heq2;rewrite abs;apply FormulaOrdered.eq_refl).
+   destruct (Maps'.find (elt:=nat) φ' Γ) .
+   rewrite MapsPtes.F.add_eq_o in u by apply FormulaOrdered.eq_refl.
+   discriminate.
+   rewrite MapsPtes.F.add_eq_o in u by apply FormulaOrdered.eq_refl.
+   discriminate.
+
+   case (FormulaOrdered.eq_dec φ' φ'');intros Heq2.
+   rewrite MapsPtes.F.add_eq_o in u by (symmetry;assumption).
+   rewrite MapsPtes.F.add_eq_o in u by apply FormulaOrdered.eq_refl.
+   discriminate.   
+   rewrite MapsPtes.F.add_neq_o in u by (intros abs;elim Heq2;rewrite abs;apply FormulaOrdered.eq_refl).
+   destruct (Maps'.find (elt:=nat) φ' Γ) .
+   rewrite MapsPtes.F.add_eq_o in u by apply FormulaOrdered.eq_refl.
+   discriminate.
+   rewrite MapsPtes.F.add_eq_o in u by apply FormulaOrdered.eq_refl.
+   discriminate.
+ Qed.
 
 
+   
+ Lemma union_singleton_decompose : 
+   ∀ Δ Δ' φ, Δ∪Δ' == {φ} -> (Δ=={φ}/\Δ'==∅)\/(Δ'=={φ}/\Δ==∅).
+ Proof.
+   intros Δ Δ' φ H.
+   destruct (env_decomp Δ).
+   right;split;auto.
+   rewrite H0 in H;exact H.
+   destruct H0 as [φ' [Γ' H1]].
+   destruct (env_decomp Γ').
+   rewrite H0 in H1;clear H0.
+   left.
+   destruct (env_decomp Δ').
+   split;auto.   
+   rewrite H1 in H;rewrite H0 in H;rewrite H1;
+   rewrite union_empty_right in H;auto.
+   destruct H0 as [φ'' [Γ'' H2]].
+   apply False_ind.   
+   rewrite H1 in H;rewrite H2 in H.
+   clear -H.
+   rewrite union_rec_right in H.
+   rewrite union_rec_left in H.
+   apply add_singleton_abs with (1:=H).
+ 
+   rewrite H1 in H;clear H1.
+   destruct H0 as [φ'' [Γ'' H1]].
+   rewrite H1 in H;clear H1.
+   rewrite union_rec_left in H.
+   rewrite union_rec_left in H.
+   elim add_singleton_abs with (1:=H).
+ Qed.
 
-
-
-
-
-
-
-
-
-
-
-
-
-
-
-(*
-Goal forall (p:  {P&1, R, G, B&1, !(V⊸A), (E⊸A)&1, (P⊸M)&1,(R⊸1)&(R⊸E), (G⊸1)⊕(G⊸V), 1⊕((B⊸V)&(B⊸1))  } ⊢ A ⊕ M), forall_impl_l_on_formula (exists_oplus_on_formula (G⊸1) (G⊸V)) R E _ _ p = true.
+Goal forall (p:{ (V⊸A),V}⊢A⊕M), 
+  exists_AtheseA_on_formula (fun _ _ _ => trueP) A M _ _ p  = trueP.
 Proof.
   intros p.
-(* inversion *)
+  
+  Ltac toto p := 
+    (dependent simple inversion p||inversion p);clear p;subst;try discriminate;simpl;
+    repeat 
+      match goal with 
+        | H : ?s == ?t |- _ => 
+          (complete (apply eq_bool_complete in H;vm_compute in H;discriminate))|| (progress repeat (rewrite H in *))
+        | H: _ ∈ (add _ _) |- _ =>   destruct (mem_destruct _ _ _ H);clear H
+        | H: _ ∈ _ |- _ => complete (vm_compute in H;discriminate)
+        | H: ILLVarInt.MILL.eq _ _ |- _ => apply eq_is_eq in H; try (injection H;clear H;intros;subst)
+        | H: context C [ remove ?f ?env ] |- _ => 
+          match env with 
+            context C' [ add f ?env' ] => 
+            let e := context C' [ env' ] in 
+              setoid_replace (remove f env) with e in H by (apply eq_bool_correct;vm_compute;reflexivity)
+          end
+  end.
+  toto p.
+  
+  Focus 1.
+  symmetry in e0.
+  destruct (union_singleton_decompose _ _ _ e0) as [[h1 h2]|[h1 h2]].
+  case (exists_AtheseA_on_formula
+         (λ (e1 : env) (f1 : formula) (_ : e1 ⊢ f1), trueP) 
+         A M Δ V i).
+  reflexivity.
+  clear - i0 h2.
+  toto i0.
+  injection H0;clear H0;intros;subst;vm_compute;reflexivity.
+  injection H0;clear H0;intros;subst. 
+  apply False_ind.
+  setoid_rewrite h2 in i;clear h2.
+  toto i.
+  apply False_ind;clear - i h2.
+  rewrite h2 in i;clear h2;toto i.
+
+
+  Focus 1.
+  injection H0;clear H0;intros;subst.
+  simpl;reflexivity.
+
+  Focus 1.  
+  injection H0;clear H0;intros;subst.
+  apply False_ind.
+  toto i.
+  symmetry in H0; destruct (union_singleton_decompose _ _ _  H0) as [[h1 h2]|[h1 h2]].
+  clear - H2 h2; rewrite h2 in H2;clear h2;toto H2.
+  clear - H2 h1; rewrite h1 in H2;clear h1;toto H2.
+Qed.
+
+Goal forall (p:{P&1, B&1, (V⊸A)&1, (E⊸A)&1,(P⊸M)&1,B ⊸ 1,V}⊢A⊕M), 
+  exists_AtheseA_on_formula (fun _ _ _ => trueP) A M _ _ p  = trueP.
+wProof.
+  intros p.
+  dependent simple inversion p;clear p;subst. 
+  apply False_ind; apply eq_bool_complete in e; vm_compute in e;discriminate.
+  discriminate.
+  assert (p0=B /\ q=1).
+  admit.
+  destruct H;subst.
+  simpl.
+  clear e.
+
+  setoid_replace (remove (B ⊸ 1)
+         {P & 1, B & 1, (V ⊸ A) & 1, (E ⊸ A) & 1, (P ⊸ M) & 1, B ⊸ 1, V}) with ({P & 1, B & 1, (V ⊸ A) & 1, (E ⊸ A) & 1, (P ⊸ M) & 1, V}) in e0 by (vm_compute;reflexivity). 
+
+
+Qed.
+Goal forall (p:  {P&1, R, G, B&1,  (V⊸A)&1, (E⊸A)&1, (P⊸M)&1,(R⊸1)&(R⊸E), (G⊸1)⊕(G⊸V), 1⊕((B⊸V)&(B⊸1))  } ⊢ A ⊕ M), forall_impl_l_on_formula (exists_oplus_on_formula (G⊸1) (G⊸V)) R E _ _ p = trueP.
+Proof.
+  intros p.
+  dependent simple inversion p;clear p;subst. 
+  apply FalseP_ind; apply eq_bool_complete in e; vm_compute in e;discriminate.
+  discriminate.
+  vm_compute in e;discriminate.
+  discriminate.
+  vm_compute in e;discriminate.
+  apply FalseP_ind; apply eq_bool_complete in e; vm_compute in e;discriminate.
+  vm_compute in e;discriminate.
+  discriminate.
+  assert (List.In (p0&q) ((P & 1)::(B&1)::((V⊸A)&1)::((E⊸A)&1)::((P⊸A)&1)::nil))%list.
+  clear -e.
+  case (FormulaOrdered.eq_dec p0 P);intros;[subst|].
+  case (FormulaOrdered.eq_dec q 1);intros;[subst|].
+  unfold mem  in e.
+  rewrite  eq_is_eq in e0;rewrite eq_is_eq in e1.
+  subst.
+  simpl;auto.
+  rewrite  eq_is_eq in e0.
+  rewrite eq_is_eq in e1.
+  admit.
+  admit.
+  admit.
+  injection H0;clear H0;intros;subst.
+  admit.
+  injection H0;clear H0;intros;subst.
+  admit.
+  discriminate.
+  vm_compute in e;discriminate.
+  vm_compute in e;discriminate.
+  vm_compute in e;discriminate.
+  vm_compute in e;discriminate.
 Qed.
 *)
 (*
@@ -313,7 +575,7 @@ Abort.
 
 
 
-
+(*
 Inductive Iexists (pred:∀ (e:env) (f:formula) (h: e ⊢ f), Prop): ∀ (e:env) (f:formula)(h: e ⊢ f) , Prop := 
 (* | IId: ∀ (f:formula) , pred {f} f (Id f) → Iexists pred {f} f (Id f) *)
 | IImpl_R: ∀ Γ p q (h:(p :: Γ ⊢ q)), Iexists pred _ _ h → Iexists pred _ _ (Impl_R Γ p q h)
@@ -360,4 +622,5 @@ Qed.
 Definition athesea' := fun e f (h:e⊢f) => (e=={f} /\ f = B).
 Lemma ata_orig': Iexists athesea' _ _ originelle.
   repeat progress constructor.
+*)
 *)
