multiset_spec.v
@@ -13,7 +13,7 @@ Module Type S(X:OrderedType).
 
   Parameter add : A -> t -> t. 
 
-  (* Parameter remove : A -> t -> option t. *)
+  Parameter remove : A -> t -> t. 
 
   Parameter mem : A -> t -> bool. 
 
@@ -28,11 +28,8 @@ Module Type S(X:OrderedType).
 
   Parameter eq_trans : forall ms1 ms2 ms3, eq ms1 ms2 -> eq ms2 ms3 -> eq ms1 ms3.
 
-  Parameter add_morph_eq : forall a a', X.eq a a' -> forall ms ms',  eq ms ms' -> eq (add a ms) (add a' ms'). 
 
   Parameter union : t -> t -> t.
-
-  Parameter union_morph_eq : forall a a', eq a a' -> forall ms ms',  eq ms ms' -> eq (union a ms) (union a' ms'). 
 
   Parameter is_empty_empty : is_empty empty = true.
   
@@ -40,23 +37,38 @@ Module Type S(X:OrderedType).
 
   Parameter add_is_not_empty : forall a ms, is_empty (add a ms) = false.
   
-  Parameter add_is_mem : forall a ms, mem a (add a ms) = true.
+  Parameter add_is_mem : forall a b ms, X.eq a b -> mem a (add b ms) = true.
+
+  Parameter mem_destruct : forall a b ms, mem a (add b ms) = true -> X.eq a b \/ mem a ms = true.
 
   Parameter add_comm : forall a b ms, eq (add a (add b ms)) (add b (add a ms)).
 
-  (* Parameter remove_mem : forall a ms, mem a ms = true -> exists ms', remove a ms = Some ms'. *)
-  (* Parameter remove_not_mem : forall a ms, mem a ms = false -> remove a ms = None. *)
- 
   Parameter mem_add_comm : forall a b ms, mem a ms = true -> mem a (add b ms) = true.
 
-  
   Parameter union_empty_left : forall ms, eq (union empty ms) ms.
   Parameter union_empty_right : forall ms, eq (union ms empty) ms.
   Parameter union_rec_left : forall a ms ms', eq (union (add a ms) ms') (add a (union ms ms')).
   Parameter union_rec_right : forall a ms ms', eq (union ms (add a ms')) (add a (union ms ms')).
 
+  Parameter remove_empty : forall φ, remove φ empty = empty.
+  Parameter remove_same_add : forall φ φ' Γ, X.eq φ φ' ->  eq (remove φ (add φ' Γ)) Γ.
+  Parameter remove_diff_add : forall φ φ' Γ, ~X.eq φ φ' -> 
+    eq (remove φ (add φ' Γ))  (add φ' (remove φ Γ)).
+
+  Parameter is_empty_morph_eq : forall (Γ Γ' : t), eq Γ Γ' -> is_empty Γ = is_empty Γ'.
+  Parameter add_morph_eq : 
+    forall a a', X.eq a a' -> forall ms ms',  eq ms ms' -> eq (add a ms) (add a' ms'). 
+  Parameter remove_morph_eq : 
+    forall a a', X.eq a a' -> forall ms ms',  eq ms ms' -> eq (remove a ms) (remove a' ms'). 
   Parameter mem_morph_eq :
     forall (φ : A) (Γ Γ' : t), eq Γ Γ' -> mem φ Γ = mem φ Γ'.
+  Parameter union_morph_eq : forall a a', eq a a' -> forall ms ms',  eq ms ms' -> eq (union a ms) (union a' ms'). 
+
+  Parameter mem_union_l : forall a ms ms', mem a ms = true -> mem a (union ms ms') = true.
+
+  Parameter mem_union_r : forall a ms ms', mem a ms' = true -> mem a (union ms ms') = true.
+
+  Parameter mem_union_destruct : forall a ms ms', mem a (union ms ms') = true -> mem a ms = true \/mem a ms' = true.
 
 End S.
 
